json: Clean up encoder and add decoder

src/JSON/JSON.AST.dfy
@@ -1,11 +1,11 @@
 module {:options "-functionSyntax:4"} JSON.AST {
-  datatype KV = KV(k: string, v: Value)
-  datatype Decimal = Decimal(n: int, e10: nat) // (n) * 10^(e10)
-  datatype Value =
+  datatype Decimal =
+    Decimal(n: int, e10: int) // (n) * 10^(e10)
+  datatype JSON =
     | Null
     | Bool(b: bool)
     | String(str: string)
     | Number(num: Decimal)
-    | Object(obj: seq<KV>) // Not a map to preserve order
-    | Array(arr: seq<Value>)
+    | Object(obj: seq<(string, JSON)>) // Not a map to preserve order
+    | Array(arr: seq<JSON>)
 }
