src/JSON/Str.dfy
@@ -1,7 +1,17 @@
 include "../BoundedInts.dfy"
+include "../Wrappers.dfy"
 
 module {:options "-functionSyntax:4"} Str {
-  module Private {
+  import opened Wrappers
+
+  abstract module ParametricConversion {
+    import opened Wrappers
+
+    type Char(==)
+    type String = seq<Char>
+
+    // FIXME the design in LittleEndianNat makes BASE a module-level constant
+    // instead of a function argument
     function Digits(n: int, base: int): (digits: seq<int>)
       requires base > 1
       requires n >= 0
@@ -18,37 +28,136 @@ module {:options "-functionSyntax:4"} Str {
         Digits(n / base, base) + [n % base]
     }
 
-    function OfDigits(digits: seq<int>, chars: seq<char>) : string
+    function OfDigits(digits: seq<int>, chars: seq<Char>) : (str: String)
       requires forall d | d in digits :: 0 <= d < |chars|
+      ensures forall c | c in str :: c in chars
     {
-      if digits == [] then ""
+      if digits == [] then []
       else
         assert digits[0] in digits;
         assert forall d | d in digits[1..] :: d in digits;
         [chars[digits[0]]] + OfDigits(digits[1..], chars)
     }
+
+    function OfNat_any(n: nat, chars: seq<Char>) : (str: String)
+      requires |chars| > 1
+      ensures forall c | c in str :: c in chars
+    {
+      var base := |chars|;
+      if n == 0 then [chars[0]]
+      else OfDigits(Digits(n, base), chars)
+    }
+
+    predicate NumberStr(str: String, minus: Char, is_digit: Char -> bool) {
+      str != [] ==>
+        && (str[0] == minus || is_digit(str[0]))
+        && forall c | c in str[1..] :: is_digit(c)
+    }
+
+    function OfInt_any(n: int, chars: seq<Char>, minus: Char) : (str: String)
+      requires |chars| > 1
+      ensures NumberStr(str, minus, c => c in chars)
+    {
+      if n >= 0 then OfNat_any(n, chars)
+      else [minus] + OfNat_any(-n, chars)
+    }
+
+    function DigitsTable(digits: seq<Char>): map<Char, nat>
+      requires forall i, j | 0 <= i < j < |digits| :: digits[i] != digits[j]
+    {
+      map i: nat | 0 <= i < |digits| :: digits[i] := i
+    }
+
+    function ToNat_any(str: String, base: nat, digits: map<Char, nat>) : (n: nat)
+      requires forall c | c in str :: c in digits
+      requires base > 0
+    {
+      if str == [] then 0
+      else ToNat_any(str[..|str| - 1], base, digits) * base + digits[str[|str| - 1]]
+    }
+
+    function ToInt_any(str: String, minus: Char, base: nat, digits: map<Char, nat>) : (s: int)
+      requires NumberStr(str, minus, c => c in digits)
+      requires str != [minus]
+      requires base > 0
+    {
+      if [minus] <= str then -(ToNat_any(str[1..], base, digits) as int)
+      else
+        assert str == [] || str == [str[0]] + str[1..];
+        ToNat_any(str, base, digits)
+    }
   }
 
-  function OfInt_any(n: int, chars: seq<char>) : string
-    requires |chars| > 1
-  {
-    var base := |chars|;
-    if n == 0 then
-      "0"
-    else if n > 0 then
-      Private.OfDigits(Private.Digits(n, base), chars)
-    else
-      "-" + Private.OfDigits(Private.Digits(-n, base), chars)
+  abstract module ParametricEscaping {
+    import opened Wrappers
+
+    type Char(==)
+    type String = seq<Char>
+
+    function Escape(str: String, special: set<Char>, escape: Char): String {
+      if str == [] then str
+      else if str[0] in special then [escape, str[0]] + Escape(str[1..], special, escape)
+      else [str[0]] + Escape(str[1..], special, escape)
+    }
+
+    datatype UnescapeError =
+      EscapeAtEOS
+
+    function Unescape(str: String, escape: Char): Result<String, UnescapeError> {
+      if str == [] then Success(str)
+      else if str[0] == escape then
+        if |str| > 1 then var tl :- Unescape(str[2..], escape); Success([str[1]] + tl)
+        else Failure(EscapeAtEOS)
+      else var tl :- Unescape(str[1..], escape); Success([str[0]] + tl)
+    }
+
+    lemma {:induction false} Unescape_Escape(str: String, special: set<Char>, escape: Char)
+      requires escape in special
+      ensures Unescape(Escape(str, special, escape), escape) == Success(str)
+    {
+      if str == [] {
+      } else {
+        assert str == [str[0]] + str[1..];
+        Unescape_Escape(str[1..], special, escape);
+      }
+    }
+  }
+
+  module CharStrConversion refines ParametricConversion {
+    type Char = char
+  }
+
+  module CharStrEscaping refines ParametricEscaping {
+    type Char = char
   }
 
   const HEX_DIGITS := [
     '0', '1', '2', '3', '4', '5', '6', '7', '8', '9',
     'A', 'B', 'C', 'D', 'E', 'F']
+  const HEX_TABLE :=
+    CharStrConversion.DigitsTable(HEX_DIGITS);
 
-  function OfInt(n: int, base: int := 10) : string
+  function OfInt(n: int, base: int := 10) : (str: string)
     requires 2 <= base <= 16
+    ensures CharStrConversion.NumberStr(str, '-', c => c in HEX_DIGITS[..base])
   {
-    OfInt_any(n, HEX_DIGITS[..base])
+    CharStrConversion.OfInt_any(n, HEX_DIGITS[..base], '-')
+  }
+
+  function ToInt(str: string, base: int := 10) : (n: int)
+    requires str != "-"
+    requires 2 <= base <= 16
+    requires CharStrConversion.NumberStr(str, '-', c => c in HEX_DIGITS[..base])
+  {
+    CharStrConversion.ToInt_any(str, '-', base, HEX_TABLE)
+  }
+
+  function EscapeQuotes(str: string): string {
+    CharStrEscaping.Escape(str, {'\"', '\''}, '\\')
+  }
+
+  function UnescapeQuotes(str: string): Result<string, CharStrEscaping.UnescapeError> {
+    CharStrEscaping.Unescape(str, '\\')
   }
 
   method Test() { // FIXME {:test}?
