src/JSON/JSON.Deserializer.dfy
@@ -1,0 +1,106 @@
+/// ===============================================
+///  Deserialization from JSON.Grammar to JSON.AST
+/// ===============================================
+///
+/// For the spec, see ``JSON.Spec.dfy``.
+
+include "../Collections/Sequences/Seq.dfy"
+include "../BoundedInts.dfy"
+include "../Math.dfy"
+
+include "Views.dfy"
+include "Vectors.dfy"
+include "UtfUtils.dfy"
+include "JSON.Errors.dfy"
+include "JSON.AST.dfy"
+include "JSON.Grammar.dfy"
+include "JSON.Spec.dfy"
+
+module {:options "-functionSyntax:4"} JSON.Deserializer {
+  import Seq
+  import Math
+
+  import opened Wrappers
+  import opened BoundedInts
+  import opened Str
+  import UtfUtils
+
+  import AST
+  import Spec
+  import opened Errors
+  import opened Vectors
+  import opened Grammar
+  import opened Views.Core
+
+  function Bool(js: Grammar.jbool): bool {
+    assert js.Bytes() in {Grammar.TRUE, Grammar.FALSE};
+    js.At(0) == 't' as byte
+  }
+
+  function Transcode8To16Unescaped(str: seq<byte>): DeserializationResult<string>
+    // TODO Optimize with a function by method
+  { // FIXME unescape unicode
+    Str.UnescapeQuotes(UtfUtils.Transcode8To16(str)).MapFailure(_ => EscapeAtEOS)
+  }
+
+  function String(js: Grammar.jstring): DeserializationResult<string> {
+    Transcode8To16Unescaped(js.Bytes())
+  }
+
+  module ByteStrConversion refines Str.ParametricConversion {
+    import opened BoundedInts
+    type Char = byte
+  }
+
+  const DIGITS := map[
+    '0' as uint8 := 0, '1' as uint8 := 1, '2' as uint8 := 2, '3' as uint8 := 3,
+    '4' as uint8 := 4, '5' as uint8 := 5, '6' as uint8 := 6, '7' as uint8 := 7,
+    '8' as uint8 := 8, '9' as uint8 := 9
+  ]
+
+  const MINUS := '-' as uint8
+
+  function ToInt(sign: jsign, n: jnum): DeserializationResult<int> {
+    var n: int := ByteStrConversion.ToNat_any(n.Bytes(), 10, DIGITS);
+    Success(if sign.Char?('-') then -n else n)
+  }
+
+  function Number(js: Grammar.jnumber): DeserializationResult<AST.Decimal> {
+    var JNumber(minus, num, frac, exp) := js;
+    var n :-
+      ToInt(minus, num);
+    var e10 :- match exp
+      case Empty => Success(0)
+      case NonEmpty(JExp(_, sign, num)) => ToInt(sign, num);
+    match frac
+      case Empty => Success(AST.Decimal(n, e10))
+      case NonEmpty(JFrac(_, num)) =>
+        var pow10 := num.Length() as int;
+        var frac :- ToInt(View.Empty, num);
+        Success(AST.Decimal(n * Math.IntPow(10, pow10) + frac, e10 - pow10))
+  }
+
+  function KV(js: Grammar.jkv): DeserializationResult<(string, AST.JSON)> {
+    var k :- String(js.k);
+    var v :- Value(js.v);
+    Success((k, v))
+  }
+
+  function Object(js: Grammar.jobject): DeserializationResult<seq<(string, AST.JSON)>> {
+    Seq.MapWithResult(d requires d in js.data => KV(d.t), js.data)
+  }
+
+  function Array(js: Grammar.jarray): DeserializationResult<seq<AST.JSON>> {
+    Seq.MapWithResult(d requires d in js.data => Value(d.t), js.data)
+  }
+
+  function Value(js: Grammar.Value): DeserializationResult<AST.JSON> {
+    match js
+      case Null(_) => Success(AST.Null())
+      case Bool(b) => Success(AST.Bool(Bool(b)))
+      case String(str) => var s :- String(str); Success(AST.String(s))
+      case Number(dec) => var n :- Number(dec); Success(AST.Number(n))
+      case Object(obj) => var o :- Object(obj); Success(AST.Object(o))
+      case Array(arr) => var a :- Array(arr); Success(AST.Array(a))
+  }
+}
