src/JSON/JSON.Errors.dfy
@@ -1,0 +1,30 @@
+include "../Wrappers.dfy"
+
+module {:options "-functionSyntax:4"} JSON.Errors {
+  import Wrappers
+
+  datatype DeserializationError =
+    | UnterminatedSequence
+    | EscapeAtEOS
+    | EmptyNumber
+    | ExpectingEOF
+    | IntOverflow
+  {
+    function ToString() : string {
+      match this
+        case EscapeAtEOS => "Escape character at end of string"
+        case UnterminatedSequence => "Unterminated sequence"
+        case EmptyNumber => "Number must contain at least one digit"
+        case ExpectingEOF => "Expecting EOF"
+        case IntOverflow => "Input length does not fit in a 32-bit counter"
+    }
+  }
+
+  datatype SerializationError =
+    | OutOfMemory
+    | IntTooLarge(i: int)
+    | StringTooLong(s: string)
+
+  type SerializationResult<+T> = Wrappers.Result<T, SerializationError>
+  type DeserializationResult<+T> = Wrappers.Result<T, DeserializationError>
+}
